@prefix dc: <http://purl.org/dc/terms/> .
@prefix dcterms: <http://purl.org/dc/terms/> .
@prefix rdf: <http://www.w3.org/1999/02/22-rdf-syntax-ns#> .
@prefix rdfs: <http://www.w3.org/2000/01/rdf-schema#> .
@prefix schema: <http://schema.org/> .
@prefix sosa: <http://www.w3.org/ns/sosa/> .
@prefix ssn-sys: <http://www.w3.org/ns/ssn/systems/> .
@prefix xml: <http://www.w3.org/XML/1998/namespace> .
@prefix xsd: <http://www.w3.org/2001/XMLSchema#> .
@prefix core: <http://schema.big-iot.org/core/> .
@prefix common: <http://schema.big-iot.org/common/> .
@prefix owl: <http://www.w3.org/2002/07/owl#>.
@prefix ns: <http://creativecommons.org/ns#>.
@prefix ssn: <http://purl.oclc.org/NET/ssnx/ssn#>.
@prefix geo: <http://www.w3.org/2003/01/geo/wgs84_pos#>.
@prefix qudt: <http://data.qudt.org/qudt/owl/1.0.0/unit.owl#>.
@prefix dul: <http://www.loa.istc.cnr.it/ontologies/DUL.owl#>.
@prefix time: <http://www.w3.org/2006/time#>.
@prefix vann: <http://purl.org/vocab/vann/>.



common: dc:contributor "Achille Zappa, NUIG, Galway"@en,
                           "Hoan Quoc, NUIG, Galway"@en,
                           "Victor Charpenay, Siemens AG, Munich"@en,
                           "Aparna Saisree, Siemens AG, Munich"@en,
                           "Darko Anicic, Siemens AG, Munich"@en,
                           "Yulia Svetashova, Bosch CR, Stutgard"@en;
                           
            dc:description " Common Model for Domain-Independent terminology annotations. We further acknowledge, Pilot providers and other open call projects for their valuable comments. Please report any errors to achille.zappa@insight-centre.org. "@en;
            dc:rights "Copyright (c) 2016-2018 by NUIGalway  (Insight Centre), Siemens, Bosch";
            dc:title "BIG IoT Common Model"@en;
            dcterms:issued "2016-09-28"^^xsd:date;
            dcterms:modified "2018-10-27"^^xsd:date;
            vann:preferredNamespacePrefix "common";
            vann:preferredNamespaceUri "http://schema.big-iot.org/common/#";
            a owl:Ontology;
            rdfs:comment " Common Model for Domain-Independent terminology annotations.  We further acknowledge, Pilot providers and other open call projects for their valuable comments. Please report any errors to achille.zappa@insight-centre.org. "@en;
            rdfs:label "BIG IoT"^^xsd:string;
            owl:versionInfo "3.0".
            
            
            
            

common:Measurement rdf:type rdfs:Class ;
  rdfs:label "Measurement" ;
  rdfs:comment "Single measurement of a physical quantity. A measurement relates to a physical quantity via the class sosa:Observation." ;
  dcterms:source <https://w3id.org/saref#Measurement> ;
  dcterms:source <http://www.wurvoc.org/vocabularies/om-1.8/Measure> ;
  dcterms:source <http://qudt.org/1.1/schema/qudt#QuantityValue> ;
  rdfs:subClassOf sosa:Result ;
.

common:BooleanMeasurement rdf:type rdfs:Class ;
  rdfs:label "Count" ;
  rdfs:comment "Measurement whose value is either 'yes' or 'no' (e.g. presence detection, status update, etc.)." ;
  rdfs:subClassOf common:Measurement ;
.

common:UnitOfMeasurement rdf:type rdfs:Class ;
  rdfs:label "UnitOfMeasurement" ;
  rdfs:comment "Unit of measurement" ;
  dcterms:source <https://w3id.org/saref#UnitOfMeasure> ;
  dcterms:source <http://www.wurvoc.org/vocabularies/om-1.8/Unit_of_measure> ;
  rdfs:subClassOf schema:Enumeration ;
.

common:degreeCelsius rdf:type common:UnitOfMeasurement ;
  rdfs:label "degreeCelsius" ;
  rdfs:comment "Degree Celsius temperature unit (symbol: Â°C)" ;
  dcterms:source <http://www.wurvoc.org/vocabularies/om-1.8/degree_Celsius> ;
.

common:kelvin rdf:type common:UnitOfMeasurement ;
  rdfs:label "kelvin" ;
  rdfs:comment "Kelvin temperature unit (symbol: K)" ;
  dcterms:source <http://www.wurvoc.org/vocabularies/om-1.8/kelvin> ;
.

common:watt rdf:type common:UnitOfMeasurement ;
  rdfs:label "watt" ;
  rdfs:comment "Watt power unit (symbol: W)" ;
  dcterms:source <http://www.wurvoc.org/vocabularies/om-1.8/watt> ;
.

common:ampere rdf:type common:UnitOfMeasurement ;
  rdfs:label "ampere" ;
  rdfs:comment "Ampere electric current unit (symbol: A)" ;
  dcterms:source <http://www.wurvoc.org/vocabularies/om-1.8/ampere> ;
.

common:volt rdf:type common:UnitOfMeasurement ;
  rdfs:label "volt" ;
  rdfs:comment "Volt electric potential difference unit (symbol: V)" ;
  dcterms:source <http://www.wurvoc.org/vocabularies/om-1.8/volt> ;
.

common:ppm rdf:type common:UnitOfMeasurement ;
  rdfs:label "ppm" ;
  rdfs:comment "parts per million unit" ;
  dcterms:source <http://www.wurvoc.org/vocabularies/om-1.8/parts_per_million> ;
.

common:gm3 rdf:type common:UnitOfMeasurement ;
  rdfs:label "gm3" ;
  rdfs:comment "concentration unit (symbol: g.m^-3)" ;
  dcterms:source <http://www.wurvoc.org/vocabularies/om-1.8/gram_per_cubic_metre> ;
.

common:percent rdf:type common:UnitOfMeasurement ;
  rdfs:label "percent" ;
  rdfs:comment "Percentage unit (symbol: %)" ;
  dcterms:source <http://www.wurvoc.org/vocabularies/om-1.8/percent> ;
.

common:decibel rdf:type common:UnitOfMeasurement ;
  rdfs:label "decibel" ;
  rdfs:comment "Arbitrary ratio unit, mostly used for sound pressure level (symbol: dB)" ;
  dcterms:source <http://www.wurvoc.org/vocabularies/om-1.8/ratio> ;
.

common:PhysicalQuantity rdf:type rdfs:Class ;
  rdfs:label "PhysicalQuantity" ;
  rdfs:comment "Measurable physical quantity (e.g. temperature, electric current, etc.)" ;
  dcterms:source <http://www.wurvoc.org/vocabularies/om-1.8/Quantity> ;
  rdfs:subClassOf sosa:Property ;
.

common:quantityUnit rdf:type rdf:Property ;
  rdfs:label "quantity unit" ;
  rdfs:comment "Unit to specify immanent characteristics (maximum current available at the charging station) as opposed to measurements." ;
  schema:domainIncludes common:PhysicalQuantity ;
  schema:rangeIncludes common:UnitOfMeasurement, schema:Text .
  
common:quantityValue rdf:type rdf:Property ;
  rdfs:label "quantity value" ;
   rdfs:comment "Value to specify immanent characteristics (maximum current available at the charging station) as opposed to measurements." ;
  schema:domainIncludes common:PhysicalQuantity ;
  schema:rangeIncludes schema:Number .

common:Temperature rdf:type rdfs:Class ;
  rdfs:label "Temperature" ;
  rdfs:comment "Temperature of a physical body" ;
  dcterms:source <http://www.wurvoc.org/vocabularies/om-1.8/Temperature> ;
  dcterms:source <https://w3id.org/saref#Temperature> ;
  rdfs:subClassOf common:PhysicalQuantity ;
.

common:Concentration rdf:type rdfs:Class ;
  rdfs:label "Concentration" ;
  rdfs:comment "Amount of substance in a given volume of some physical body" ;
  dcterms:source <http://www.wurvoc.org/vocabularies/om-1.8/Amount_of_substance_concentration> ;
  rdfs:subClassOf common:PhysicalQuantity ;
.

common:Speed rdf:type rdfs:Class ;
  rdfs:label "Speed" ;
  rdfs:comment "Speed (distance divided by time) of a physical body." ;
  dcterms:source <http://www.wurvoc.org/vocabularies/om-1.8/Speed> ;
  rdfs:subClassOf common:PhysicalQuantity ;
.

common:Percentage rdf:type rdfs:Class ;
  rdfs:label "Percentage" ;
  rdfs:comment "Ratio of a quantity value divided by hundred." ;
  dcterms:source <http://www.wurvoc.org/vocabularies/om-1.8/Percentage> ;
  rdfs:subClassOf common:PhysicalQuantity ;
.

common:Count rdf:type rdfs:Class ;
  rdfs:label "Count" ;
  rdfs:comment "Count of all individuals of a countable concept." ;
  dcterms:source <http://www.wurvoc.org/vocabularies/om-1.8/Number> ;
  rdfs:subClassOf common:PhysicalQuantity ;
.

common:Power rdf:type rdfs:Class ;
  rdfs:label "Power" ;
  rdfs:comment "Power is energy divided by time (often expressed in Watt)" ;
  dcterms:source <http://www.wurvoc.org/vocabularies/om-1.8/Power> ;
  dcterms:source <https://w3id.org/saref#Power> ;
  rdfs:subClassOf common:PhysicalQuantity ;
.

common:ElectricCurrent rdf:type rdfs:Class ;
  rdfs:label "ElectricCurrent" ;
  rdfs:comment "Electric current is the flow of electric charge (often expressed in Ampere)" ;
  dcterms:source <http://www.wurvoc.org/vocabularies/om-1.8/Electric_current> ;
  rdfs:subClassOf common:PhysicalQuantity ;
.

common:VoltageOrPotentialDifference rdf:type rdfs:Class ;
  rdfs:label "VoltageOrPotentialDifference" ;
  rdfs:comment "Voltage is the electric potential difference between two points of a circuit (often expressed in Volt)" ;
  dcterms:source <http://www.wurvoc.org/vocabularies/om-1.8/Potential_difference> ;
  rdfs:subClassOf common:PhysicalQuantity ;
.

common:unit rdf:type rdf:Property ;
  rdfs:label "unit" ;
  rdfs:comment "A measurement consists of a pair (value, unit)." ;
  dcterms:source <http://www.wurvoc.org/vocabularies/om-1.8/unit_of_measure_or_measurement_scale> ;
  dcterms:source <http://qudt.org/1.1/schema/qudt#unit> ;
  schema:domainIncludes common:Measurement ;
  schema:rangeIncludes common:UnitOfMeasurement ;
.

common:numericValue rdf:type rdf:Property ;
  rdfs:label "numericValue" ;
  rdfs:comment "A measurement consists of a pair (value, unit)." ;
  dcterms:source <http://www.wurvoc.org/vocabularies/om-1.8/numerical_value> ;
  dcterms:source <http://qudt.org/1.1/schema/qudt#numericValue> ;
  schema:domainIncludes common:Measurement ;
  schema:rangeIncludes schema:Number ;
.
    
common:Accuracy
  rdf:type rdfs:Class ;
  dcterms:source <http://www.w3.org/ns/ssn/systems/Accuracy> ;
  rdfs:label "Accuracy"^^xsd:string ;
  rdfs:comment "See https://www.w3.org/TR/vocab-ssn/#SSNSYSTEMAccuracy."^^xsd:string ;
  rdfs:subClassOf common:SystemProperty ;
.
common:SystemProperty
  rdf:type rdfs:Class ;
  dcterms:source <http://www.w3.org/ns/ssn/systems/SystemProperty> ;
  rdfs:label "SystemProperty"^^xsd:string ;
  rdfs:comment "See https://www.w3.org/TR/vocab-ssn/#SSNSYSTEMSystemProperty."^^xsd:string ;
  rdfs:subClassOf core:BasicData ;
.

# TODO 'accuracy' should be better aligned with SSN

common:accuracy rdf:type rdf:Property ;
  rdfs:label "accuracy" ;
  rdfs:comment "Accuracy of a measurement" ;
  schema:domainIncludes common:Measurement ;
  schema:rangeIncludes common:Accuracy ;
  dcterms:source <http://www.w3.org/ns/ssn/systems/hasSystemProperty> ;
.

common:Box
  rdf:type rdfs:Class ;
  common:hasCorners common:Corners ;
  rdfs:label "Bounding Box"^^xsd:string ;
  rdfs:subClassOf core:BasicData ;
  rdfs:subClassOf schema:Geoshape ;
.

common:Corners
  rdf:type rdfs:Class ;
  common:hasNorthEastCornor schema:GeoCoordinates ;
  common:hasSouthWestCornor schema:GeoCoordinates ;
  rdfs:label "Corners"^^xsd:string ;
  rdfs:subClassOf core:BasicData ;
.
  
common:Polygon
  rdf:type rdfs:Class ;
  rdfs:label "Polygon"^^xsd:string ;
  rdfs:comment "A polygon."^^xsd:string ;
  rdfs:subClassOf schema:Geoshape ;
  rdfs:subClassOf core:BasicData ;
.

common:mile rdf:type common:UnitOfMeasurement ;
  rdfs:label "mile" ;
  rdfs:comment "A unit of visibility defined as mile (mi)."  .
  
common:kilometre rdf:type common:UnitOfMeasurement ;
  rdfs:label "kilometre" ;
  rdfs:comment "A unit of visibility defined as kilometre (km)."  . 

common:centimetre rdf:type common:UnitOfMeasurement ;
  rdfs:label "centimetre" ;
  rdfs:comment "A unit defined as centimetre (cm)."  .    

common:millimetre rdf:type common:UnitOfMeasurement ;
  rdfs:label "millimetre" ;
  rdfs:comment "A unit of rainfall defined as millimetre (mm)."  .  
  
common:okta rdf:type common:UnitOfMeasurement ;
  rdfs:label "okta" ;
  rdfs:comment "An okta is a unit of measurement used to describe the amount of cloud cover at any given location such as a weather station."  .    
  
common:kilometrePerHour rdf:type common:UnitOfMeasurement ;
  rdfs:label "kilometrePerHour" ;
  rdfs:comment "A unit of speed defined as kilometre divided by hour." ;
  dcterms:source <http://www.wurvoc.org/vocabularies/om-1.8/kilometre_per_hour> .

common:litrePerHour rdf:type common:UnitOfMeasurement ;
  rdfs:label "litrePerHour" ;
  rdfs:comment "A unit of volume flow rate defined as liters divided by hour." ;
  dcterms:source <http://www.wurvoc.org/vocabularies/om-1.8/litre_per_hour> .

common:kilogramPerHour rdf:type common:UnitOfMeasurement ;
  rdfs:label "kilogramPerHour" ;
  rdfs:comment "A unit of mass flow rate defined as kilogram divided by hour." ;
  dcterms:source <http://www.qudt.org/qudt/owl/1.0.0/unit/Instances.html#KilogramPerHour> .

common:gramPerSecond rdf:type common:UnitOfMeasurement ;
  rdfs:label "gramPerSecond" ;
  rdfs:comment "A unit of mass flow rate defined as gram divided by second." .

common:kiloPascal rdf:type common:UnitOfMeasurement ;
  rdfs:label "kiloPascal" ;
  rdfs:comment "A unit of pressure or stress (1 kPa = 1000 Pa)." ;
  dcterms:source <http://www.qudt.org/qudt/owl/1.0.0/unit/Instances.html#KiloPascal> .

common:kiloPascalAbsolute rdf:type common:UnitOfMeasurement ;
  rdfs:label "kiloPascalAbsolute" ;
  rdfs:comment "A unit of pressure or stress (1 kPa = 1000 Pa) measured from absolute zero." ;
  dcterms:source <http://www.qudt.org/qudt/owl/1.0.0/unit/Instances.html#KiloPascalAbsolute> .

common:revolutionPerMinute rdf:type common:UnitOfMeasurement ;
  rdfs:label "revolutionPerMinute (rpm)" ;
  rdfs:comment "A unit of frequency of rotation, specifically the number of rotations around a fixed axis in one minute." ;
  dcterms:source <http://www.qudt.org/qudt/owl/1.0.0/unit/Instances.html#RevolutionPerMinute> .

common:milliampere rdf:type common:UnitOfMeasurement ;
  rdfs:label "milliampere" ;
  rdfs:comment "A unit of electric current defined as 1.0e-3 ampere (symbol: mA)" ;
  dcterms:source <http://www.wurvoc.org/vocabularies/om-1.8/milliampere> .

common:metre rdf:type common:UnitOfMeasurement ;
  rdfs:label "metre" ;
  rdfs:comment "A unit of length (symbol: m)" ;
  dcterms:source <http://www.wurvoc.org/vocabularies/om-1.8/metre> .

common:degree rdf:type common:UnitOfMeasurement ;
  rdfs:label "degree" ;
  rdfs:comment "A unit of plane angle defined as 1.745329e-2 radian." ;
  dcterms:source <http://www.wurvoc.org/vocabularies/om-1.8/degree> .

common:sensorID a rdf:Property ;
    rdfs:label "sensorID"^^xsd:string ;
    rdfs:comment "The identifier of a sensor." ;
    dc:source <http://schema.org/identifier> ;
    schema:domainIncludes sosa:Sensor ;
    schema:rangeIncludes schema:Text .

common:sensorURL a rdf:Property ;
    rdfs:label "sensorURL"^^xsd:string ;
    rdfs:comment "The URL of a sensor." ;
    dc:source <http://schema.org/identifier> ;
    schema:domainIncludes sosa:Sensor ;
    schema:rangeIncludes schema:URL .

common:measurementID a rdf:Property ;
    rdfs:label "measurementID"^^xsd:string ;
    rdfs:comment "The identifier of a measurement." ;
    dc:source <http://schema.org/identifier> ;
    schema:domainIncludes sosa:Observation ;
    schema:rangeIncludes schema:Text .

common:measurementURL a rdf:Property ;
    rdfs:label "measurementURL"^^xsd:string ;
    rdfs:comment "The URL of a measurement." ;
    dc:source <http://schema.org/identifier> ;
    schema:domainIncludes sosa:Observation ;
    schema:rangeIncludes schema:URL .
    
common:measurementTime a rdf:Property ;
  rdfs:label "measurement time"^^xsd:string ;
  rdfs:comment "Measurement time stamp: date and time."^^xsd:string ;
  dc:source <http://www.w3.org/ns/sosa/resultTime> ;
  schema:domainIncludes common:Measurement ;
  schema:rangeIncludes schema:DateTime .
  
common:measurementDate a rdf:Property ;
  rdfs:label "measurement date"^^xsd:string ;
  rdfs:comment "Measurement date."^^xsd:string ;
  schema:domainIncludes common:Measurement ;
  schema:rangeIncludes schema:DateTime .
    
common:pageNumber a rdf:Property ;
    rdfs:label "page number"^^xsd:string ;
    rdfs:comment "Page number indicates the position in the set of all entities returned as the response to a request." ;
    schema:domainIncludes core:BasicData ;
    schema:rangeIncludes schema:Number .
    
# Proposed: SOSA alignment-related modeling
common:PropertyType rdf:type rdfs:Class ;
  rdfs:label "Annotation type" ;
  rdfs:comment "Type of a property annotation." .

common:TemporalProperty rdf:type rdfs:Class ;
	rdfs:label	"Temporal property" ;
	rdfs:comment	"Time-related properties." ;
	rdfs:subClassOf common:PropertyType .

common:SpatialProperty rdf:type rdfs:Class ;
	rdfs:label	"Spatial property" ;
	rdfs:comment	"Location-related properties." ;
	rdfs:subClassOf common:PropertyType .
	
common:ObservableProperty rdf:type rdfs:Class ;
	rdfs:label	"Observable property" ;
	rdfs:comment	"Dynamic (changing) properties." ;
	rdfs:subClassOf common:PropertyType .
	
common:StaticProperty rdf:type rdfs:Class ;
	rdfs:label	"Static property" ;
	rdfs:comment	"Static (non-changing) properties." ;
	rdfs:subClassOf common:PropertyType .
 
common:propertyType a rdf:Property ;
    rdfs:label "property type"^^xsd:string ;
    rdfs:comment "Used to annotate properties in the domain models as representing temporal, spatial, dynamic or static properties of classes." ;
    schema:domainIncludes rdf:Property ;
    schema:rangeIncludes common:PropertyType .
    
common:geoJSONLocation  a rdf:Property ;
    rdfs:label "GeoJSON location"^^xsd:string ;
    rdfs:comment "GeoJSON geometry object representing points, curves, and surfaces in coordinate space." ;
    schema:domainIncludes schema:Place ;
	schema:rangeIncludes common:GeoJSONGeometryObject .

common:GeoJSONGeometryObject rdf:type rdfs:Class ;
	rdfs:label	"GeoJSON Geometry Object" ;
	rdfs:comment	"A GeoJSON object that represents points, curves, and surfaces in coordinate space." ;
	rdfs:isDefinedBy <https://tools.ietf.org/html/rfc7946#section-3.1> .
	
common:geoJSONLocationType a rdf:Property ;
	rdfs:label "GeoJSON location type" ;
	rdfs:comment "GeoJSON geometry object type: Point, LineString, Polygon, MultiPoint, MultiLineString, MultiPolygon, and GeometryCollection" ;
    schema:domainIncludes common:GeoJSONGeometryObject ;
	schema:rangeIncludes schema:Text .

common:geoJSONLocationCoordinates a rdf:Property ;
	rdfs:label "GeoJSON location coordinates" ;
	rdfs:comment "An array of coordinates. The structure of the elements in this array is determined by the type of geometry." ;
	schema:domainIncludes common:GeoJSONGeometryObject ;
	schema:rangeIncludes schema:Text, schema:Number .
	
common:street a rdf:Property ;
	rdfs:label "street" ;
	rdfs:comment "Street without a house number." ;
    schema:domainIncludes schema:PostalAddress;
	schema:rangeIncludes schema:Text .

common:houseNumber a rdf:Property ;
	rdfs:label "house number" ;
	rdfs:comment "A house number." ;
    schema:domainIncludes schema:PostalAddress;
	schema:rangeIncludes schema:Text .

common:district a rdf:Property ;
	rdfs:label "district" ;
	rdfs:comment "District in a city." ;
    schema:domainIncludes schema:PostalAddress;
	schema:rangeIncludes schema:Text .

common:featureType a rdf:Property ;
	# find a more precise definition and a domain for that property
	rdfs:label "feature type" ;
	rdfs:comment "Property that helps to define the scope of the hierarchically organized JSON objects, e.g. [Charging Station has [ChargingPoint [has Plug]]]" ;
	schema:rangeIncludes schema:Text .

schema:telephone schema:rangeIncludes schema:Number .

common:CrowdsourcingData a rdfs:Class ;
	rdfs:subClassOf sosa:FeatureOfInterest ;
	rdfs:label "CrowdsourcingData" ;
	rdfs:comment "Class to manage survey responses collected via crowdsourcing." .
	
common:Survey a rdfs:Class ;
	rdfs:subClassOf common:CrowdsourcingData ;
	rdfs:label "Survey" ;
	rdfs:comment "Survey conducted by using crowdsourcing techniques." .
	
common:hasSurveyResponse a rdf:Property ;
    rdfs:label "survey response" ;
    rdfs:comment "One response to a survey." ;
    schema:domainIncludes common:Survey ;
    schema:rangeIncludes common:SurveyResponse .
	
common:SurveyResponse a rdfs:Class ;
	rdfs:label "SurveyResponse" ;
	rdfs:comment "One response to a survey." .

common:question a rdf:Property ;
	rdfs:label "question" ;
	rdfs:comment "Question in a survey to which a response is acquired." ;
	schema:domainIncludes common:SurveyResponse ;
	schema:rangeIncludes schema:Text .
	
common:answerOptions a rdf:Property ;
	rdfs:label "answer options" ;
	rdfs:comment "Answer options (array of text strings) for a question in a survey to which a response is acquired." ;
	schema:domainIncludes common:SurveyResponse ;
	schema:rangeIncludes schema:Text .
	
common:selectedAnswerOption a rdf:Property ;
	rdfs:label "selected answer option" ;
	rdfs:comment "The number of the option selected by a respondent among the available answer options." ;
	schema:domainIncludes common:SurveyResponse ;
	schema:rangeIncludes schema:Text .